---
layout: post
title: double sum 1
tags:
  - sum  
  - closed-form
  - real-analysis
  
description:  
  double sum 1
hero: https://source.unsplash.com/collection/145103/
overlay: blue
published: true
---


# Question

Sum of :
 
 
$$
 
\sum_{k=1}^{\infty} \sum_{n=1}^{\infty} \frac{1}{n^2k^2(n+k)^2} 
 
$$
 


<!–-break-–


# Answer

We have 

$$
\begin{equation*}
\begin{aligned} 
\displaystyle 
\sum_{k=1}^{\infty} \sum_{n=1}^{\infty} \frac{1}{n^2k^2(n+k)^2} 
& = \frac{1}{3}\sum\limits_{n,k=1}^{\infty}\frac{(n+k)^3 - n^3-k^3}{n^3k^3(n+k)^3} \\ 
&= \frac{1}{3}\sum\limits_{n,k=1}^{\infty} \frac{1}{n^3k^3} - \frac{1}{3}\sum\limits_{n,k=1}^{\infty}\frac{1}{n^3(n+k)^3} - \frac{1}{3}\sum\limits_{n,k=1}^{\infty}\frac{1}{k^3(n+k)^3} \\ 
&=\frac{1}{3}\sum\limits_{n,k=1}^{\infty} \frac{1}{n^3k^3} - \frac{1}{3}\sum\limits_{n>k} \frac{1}{n^3k^3} - \frac{1}{3}\sum\limits_{n<k} \frac{1}{n^3k^3} \\&= \frac{1}{3}\sum\limits_{n=k} \frac{1}{n^3k^3} \\
&=  \frac{1}{3}\zeta(6) 
\end{aligned}
\end{equation*}
$$